dataplane/Examples/Batch_op_Correctness.thy
@@ -5,36 +5,57 @@ imports
   Source_op
   Ooo_Input_op
   Batch_op
+  "../MyProduct_Instances"
 begin
 
 partial_function (llist) batch_fun_spec where
  "batch_fun_spec f lxs buf caps = (case lxs of
     LNil \<Rightarrow> (
-    let compl_batches = (\<lambda> t. filter (\<lambda> (d, t'). t' = t) buf) in
-    let outs = concat (map (\<lambda> t. map (\<lambda> x. (x, t)) (f (compl_batches t))) (rmdups {} caps)) in
-    LCons outs LNil)
-  | LCons (Data t d) lxs' \<Rightarrow> batch_fun_spec f lxs' (buf @ [(t, d)]) caps
+    let compl_batches = (\<lambda> t. map fst ((filter (\<lambda> (d, t'). t' = t)) buf)) in
+    let outs =  map (\<lambda> t. map (\<lambda> x. (x, t)) (f (compl_batches t))) (rmdups {} (map snd buf)) in
+    llist_of outs)
+  | LCons (Data t (d :: 'd1)) lxs' \<Rightarrow> batch_fun_spec f lxs' (buf @ [(d, t)]) caps
   | LCons (Mint t) lxs' \<Rightarrow> batch_fun_spec f lxs' buf (caps @ [t])
   | LCons (Drop t) lxs' \<Rightarrow> (
     let below_caps = filter (\<lambda> t. \<not> frontier_less_equal (frontier (zmset_of (mset caps - {# t #}))) t) caps in
-    let compl_batches = (\<lambda> t. filter (\<lambda> (d, t'). t' = t \<and> t' \<in> set below_caps) buf) in
-    let outs = concat (map (\<lambda> t. map (\<lambda> x. (x, t)) (f (compl_batches t))) ((rmdups {} (map snd buf)))) in
+    let compl_batches = (\<lambda> t. map fst (filter (\<lambda> (d, t'). t' = t \<and> t' \<in> set below_caps) buf)) in
+    let outs = concat (map (\<lambda> t. map (\<lambda> x. (x, t)) (f (compl_batches t))) (filter (\<lambda> t. t \<in> set below_caps) (rmdups {} (map snd buf)))) in
     let buf' = filter (\<lambda> (d, t). t \<notin> set below_caps) buf in
     LCons outs (batch_fun_spec f lxs' buf' (remove_last t caps))))"
 
+declare batch_fun_spec.simps[code]
 
+abbreviation "t1 \<equiv> MyPair (Suc 0) (0 :: nat)"
+abbreviation "t2 \<equiv> MyPair (0 :: nat) (Suc 0)"
+abbreviation "t3 \<equiv> MyPair (Suc 0) (Suc 0)"
 
-abbreviation "inp_top os inps \<equiv> map_op (case_option (Inl (0 :: 2)) (\<lambda> p. Inr (0, p))) (case_option (Inl (0 :: 2)) (\<lambda> p. Inr (0, p))) (ooo_input_op os inps)"
+value \<open>list_of (lconcat (batch_fun_spec 
+ (\<lambda> b. [Max (set b)]) (llist_of [Mint t1, Mint t2, Mint t3, Data t3 42, Data t2 7, Data t1 (-2), Data t2 (-1), Data t1 (- 3), Drop t3, Drop t1, Drop t2]) [] [] :: (int \<times> _) buf llist))\<close>
 
-abbreviation "b_op os f \<equiv> map_op (case_option (Inl (1 :: 2)) (\<lambda> p. Inr (1, p))) (case_option (Inl (1 :: 2)) (\<lambda> p. Inr (1, p))) (batch_fun_op os f)"
-
-abbreviation "inp_m_top os1 inps buf os2 f \<equiv>
+abbreviation "inp_op os \<equiv> map_op (case_option (Inl (0 :: 2)) (\<lambda> p. Inr (0, p))) (case_option (Inl (0 :: 2)) (\<lambda> p. Inr (0, p))) (ooo_input_op {|1|} os)"
+abbreviation "bt_op os f \<equiv> map_op (case_option (Inl (1 :: 2)) (\<lambda> p. Inr (1, p))) (case_option (Inl (1 :: 2)) (\<lambda> p. Inr (1, p))) (batch_fun_op os f)"
+abbreviation "inp_bt_op os1 cbuf os2 f \<equiv>
    map_op (case_sum id id) (case_sum id id)
-   (comp_op [Inr (0 :: 2, 0 :: 1) \<mapsto> Inr (1 :: 2, 0 :: 1)] buf (inp_top os1 inps) (b_op os2 f))"
+   (comp_op [Inr (0 :: 2, 0 :: 1) \<mapsto> Inr (1 :: 2, 0 :: 1)] cbuf (inp_op (os1\<lparr> en1 := Inl \<rparr>)) (bt_op (os2\<lparr> de1 := projl, en2 := Inr \<rparr>) f))"
+
+lemma dataflow_op_inp_bt_op_wbisim_source_op_aux:
+  fixes lxs :: \<open>('t :: {ccompare,canonically_ordered_monoid_add,ordered_ab_semigroup_monoid_add_imp_le}, 'd1) event llist\<close>
+  and f :: \<open>'d1 buf \<Rightarrow> 'd2 buf\<close>
+  and os1 :: \<open>(1, 'd1 + 'd2, 'd1, 't) input_state\<close>
+  and os2 :: \<open>(1, 'd1 + 'd2, 'd1, 'd2, 't) operator_state_ty2\<close>
+assumes
+  state_inv: 
+   \<open>es os1 1 = lxs\<close>
+   \<open>outpu os1 1 = map (\<lambda> (d, t). (Inl d, t)) outpos1\<close>
+   \<open>input os2 1 = map (\<lambda> (d, t). (Inl d, t)) inpos2\<close>
+   \<open>buf = outpos1 @ cbuf @ inpos\<close>
+shows 
+  \<open>dataflow_op sg (inp_bt_op os1 (\<lambda> p. case p of Inl x \<Rightarrow> [] | Inr x \<Rightarrow> map (\<lambda> (d, t). Inr (Inl d, t)) cbuf) os2 f) \<approx>
+   map_op (\<lambda> p. (1, p)) (\<lambda> p. (1, p)) (source_op (\<lambda> p. outpu os2 1 @@- lmap (\<lambda> (d, t). (Inr d, t)) (lconcat (batch_fun_spec f lxs' buf caps))))\<close>
 
 
-term "inp_m_top os1 inps buf os2 f"
+  term outpos1
+  term buf
 
-term "source_op (\<lambda> p. lconcat (batch_fun_spec f lxs buf caps))"
 
 end
